Fix examples (WIP)

examples/struct/point.pos/Test.fst
@@ -13,13 +13,15 @@ let point_struct_t = S.TStruct point_struct
 
 let point = S.pointer point_struct_t
 
+#set-options "--z3rlimit 16"
+
 let flip
   (p: point)
 : HST.Stack unit
-  (requires (fun h -> S.live h p))
+  (requires (fun h -> S.readable h p))
   (ensures (fun h0 _ h1 -> 
-      S.live h0 p
-    /\ S.live h1 p
+      S.readable h0 p
+    /\ S.readable h1 p
     /\ S.modifies_1 p h0 h1
     /\ S.gread h1 (S.gfield p "X") == S.gread h0 (S.gfield p "Y")
     /\ S.gread h1 (S.gfield p "Y") == S.gread h0 (S.gfield p "X")
@@ -30,23 +32,40 @@ let flip
   let color = S.read (S.field p "Color") in
   S.write (S.field p "X") y;
   S.write (S.field p "Y") x;
-  S.write (S.field p "Color") (not color)
+  S.write (S.field p "Color") (not color);
+  S.readable_struct_forall_mem p
 
-let flip'
+#set-options "--z3rlimit 128 --max_fuel 20 --max_ifuel 20"
+
+val flip'
   (p: point)
 : HST.Stack unit
-  (requires (fun h -> S.live h p))
+  (requires (fun h -> S.readable h p))
   (ensures (fun h0 _ h1 -> 
-      S.live h0 p
-    /\ S.live h1 p
+      S.readable h0 p
+    /\ S.readable h1 p
     /\ S.modifies_1 p h0 h1
     /\ S.gread h1 (S.gfield p "X") == S.gread h0 (S.gfield p "Y")
     /\ S.gread h1 (S.gfield p "Y") == S.gread h0 (S.gfield p "X")
     /\ S.gread h1 (S.gfield p "Color") == not (S.gread h0 (S.gfield p "Color"))
     ))
-= let x = S.read (S.field p "X") in
+let flip' p
+= assert ("X" `S.is_struct_field_of` point_struct);
+  assert ("Y" `S.is_struct_field_of` point_struct);
+  assert_norm ("Color" `S.is_struct_field_of` point_struct);
+  assume ("Color" `S.is_struct_field_of` point_struct); // FIXME: WHY WHY WHY does this assert NOT work?
+  let x = S.read (S.field p "X") in
   let y = S.read (S.field p "Y") in
   S.write (S.field p "X") y;
   S.write (S.field p "Y") x;
-  let color = S.read (S.field p "Color") in
-  S.write (S.field p "Color") (not color)
+  let h = HST.get () in
+  assume (S.readable h (S.gfield p "Color"));
+  assume (S.typ_of_struct_field point_struct "Color" == S.TBase S.TBool);
+  let color: bool = S.read (S.field p "Color") in
+  S.write (S.field p "Color") (not color);
+  let h = HST.get () in
+  assert (S.readable h (S.gfield p "X"));
+  assert (S.readable h (S.gfield p "Y"));
+  assert (S.readable h (S.gfield p "Color"));
+  assume (S.readable h p)
+//  S.readable_struct_forall_mem p
